New proposal for modular arraystruct with pcms

ulib/experimental/Steel.PCM.ArrayStruct.fst
@@ -31,274 +31,135 @@ let v_usize = U32.v
 type field_id = string
 
 noeq type array_struct_descriptor : Type u#(a+1) =
-  // You can store your own funky PCM in the Base case
-  | Base: a: Type u#a -> pcm: pcm a -> array_struct_descriptor
-  | Array: cell_descriptor:array_struct_descriptor u#a -> len:usize -> array_struct_descriptor
-  | Struct: field_descriptors: (field_id ^-> option (array_struct_descriptor u#a)) ->
+  | DBase:
+    a: Type u#a ->
+    array_struct_descriptor
+  | DArray:
+    cell_descriptor:array_struct_descriptor u#a ->
+    len:usize ->
+    array_struct_descriptor
+  | DStruct:
+    field_descriptors: (field_id ^-> array_struct_descriptor u#a) ->
     array_struct_descriptor
   // Missing: untagged unions (not must have)
 
 unfold let struct_field_type'
-  (field_descriptors: (field_id ^-> option (array_struct_descriptor u#a)))
+  (field_descriptors: (field_id ^-> array_struct_descriptor u#a))
   (array_struct_type: (descriptor: array_struct_descriptor u#a{
     descriptor << field_descriptors
   }) -> Tot (Type u#a))
   (field: field_id)
   : Tot (Type u#a) =
-  match field_descriptors field with
-      | Some descr ->
-        FStar.WellFounded.axiom1 field_descriptors field;
-        array_struct_type descr
-      | None -> Univ.raise_t u#0 u#a unit
+  let descr = field_descriptors field in
+  FStar.WellFounded.axiom1 field_descriptors field;
+  array_struct_type descr
+
+let array_type (cell_type: Type u#a) (len: usize) : Type u#a =
+  Seq.lseq cell_type (v_usize len)
+
+let struct_type (field_typs: field_id -> Type u#a) : Type u#a =
+  DepMap.t field_id field_typs
 
 let rec array_struct_type (descriptor: array_struct_descriptor u#a) : Tot (Type u#a) (decreases descriptor) =
   match descriptor with
-  | Base a pcm -> a
-  | Array descriptor' len ->
+  | DBase a -> a
+  | DArray descriptor' len ->
     let typ' = array_struct_type descriptor' in
-    Seq.lseq u#a typ' (v_usize len)
-  | Struct field_descriptors ->
-    DepMap.t field_id (struct_field_type' field_descriptors array_struct_type)
+    array_type typ' len
+  | DStruct field_descriptors ->
+    let typs' = struct_field_type' field_descriptors array_struct_type in
+    struct_type typs'
 
 unfold let struct_field_type
-  (field_descriptors: (field_id ^-> option (array_struct_descriptor u#a)))
+  (field_descriptors: (field_id ^-> (array_struct_descriptor u#a)))
   (field: field_id)
   : Tot (Type u#a) =
   struct_field_type' field_descriptors array_struct_type field
 
+noeq type array_struct_nested_pcm : Type u#(a+1) =
+  | PBase:
+    a: Type u#a ->
+    pcm: pcm a ->
+    array_struct_nested_pcm
+  | PArray:
+    cell_type: Type u#a ->
+    len: usize ->
+    cell_nested_pcm: array_struct_nested_pcm u#a ->
+    array_pcm: (pcm cell_type -> pcm (array_type cell_type len)) ->
+    array_struct_nested_pcm
+  | PStruct:
+    field_types: (field_id ^-> Type u#a) ->
+    field_nested_pcms: (field:field_id -> array_struct_nested_pcm u#a) ->
+    struct_pcm: ((field:field_id -> pcm (field_types field)) -> pcm (struct_type field_types)) ->
+    array_struct_nested_pcm
+
+let rec nested_pcm_sync
+  (descriptor: array_struct_descriptor)
+  (nested_pcm: array_struct_nested_pcm) : GTot prop (decreases descriptor) =
+  match descriptor, nested_pcm with
+  | DBase da, PBase va _ ->
+    da == va
+  | DArray cell_descriptor dlen, PArray cell_type plen cell_nested_pcm _  ->
+    dlen = plen /\ cell_type == array_struct_type cell_descriptor /\
+    cell_descriptor `nested_pcm_sync` cell_nested_pcm
+  | DStruct field_descriptors, PStruct field_types field_nested_pcms struct_pcm ->
+    field_types == struct_field_type field_descriptors /\
+    (forall (field: field_id). begin
+      FStar.WellFounded.axiom1 field_descriptors field;
+      field_descriptors field `nested_pcm_sync` field_nested_pcms field
+    end)
+  | _ -> False
+
 noeq type array_struct : Type u#(a+1) =
   | ArrayStruct:
     descriptor: array_struct_descriptor u#a ->
-    value:(array_struct_type  descriptor) -> array_struct
+    nested_pcm: array_struct_nested_pcm u#a{descriptor `nested_pcm_sync` nested_pcm} ->
+    value: array_struct_type descriptor ->
+    array_struct
 
-let struct_field_type_unroll_lemma_aux
-  (field_descriptors : (field_id ^-> option (array_struct_descriptor u#a)))
+let struct_field_type_unroll_lemma
+  (field_descriptors : (field_id ^-> array_struct_descriptor u#a))
     : Lemma (
       DependentMap.t u#a field_id (struct_field_type u#a field_descriptors) ==
-      array_struct_type u#a (Struct u#a field_descriptors)
+      array_struct_type u#a (DStruct u#a field_descriptors)
      )
   =
   let open FStar.Tactics in
   assert (
     DependentMap.t field_id (struct_field_type field_descriptors) ==
-    array_struct_type (Struct field_descriptors)
+    array_struct_type (DStruct field_descriptors)
   ) by begin
     compute ()
   end
 
-let struct_field_type_unroll_lemma
-  (s: array_struct u#a{Struct? s.descriptor})
-  : Lemma (
-    DependentMap.t u#a field_id (struct_field_type u#a (Struct?.field_descriptors s.descriptor))
-    ==
-    array_struct_type u#a s.descriptor
-  )
-  =
-  struct_field_type_unroll_lemma_aux (Struct?.field_descriptors s.descriptor)
-
-let array_cell_type_unroll_lemma_aux
-  (cell_descriptor : array_struct_descriptor u#a)
-  (len: usize)
-    : Lemma (
-      Seq.lseq (array_struct_type cell_descriptor) (v_usize len) ==
-      array_struct_type u#a (Array u#a cell_descriptor len)
-     )
-  =
-  let open FStar.Tactics in
-  assert (
-     Seq.lseq (array_struct_type cell_descriptor) (v_usize len) ==
-      array_struct_type u#a (Array u#a cell_descriptor len)
-  ) by begin
-    compute ()
-  end
-
-let array_cell_type_unroll_lemma
-  (s: array_struct u#a{Array? s.descriptor})
-    : Lemma (
-      Seq.lseq
-        (array_struct_type (Array?.cell_descriptor s.descriptor))
-        (v_usize (Array?.len s.descriptor)) ==
-      array_struct_type u#a s.descriptor
-     )
-  =
-  array_cell_type_unroll_lemma_aux
-    (Array?.cell_descriptor s.descriptor)
-    (Array?.len s.descriptor)
-
-
-let array_cell_sub_array_struct
-  (s: array_struct u#a{Array? s.descriptor})
-  (i:nat{i < v_usize (Array?.len s.descriptor)})
-  : Tot (s':array_struct u#a{s'.descriptor << s.descriptor})
-  =
-  let cell_descriptor = Array?.cell_descriptor s.descriptor in
-  let len = Array?.len s.descriptor in
-  array_cell_type_unroll_lemma s;
-  let v: Seq.lseq u#a (array_struct_type u#a cell_descriptor) (v_usize len) = s.value in
-  let sub_v = Seq.index u#a v i in
-  ArrayStruct u#a cell_descriptor sub_v
-
-let struct_field_sub_array_struct
-  (s: array_struct u#a{Struct? s.descriptor})
-  (field: field_id{Some? ((Struct?.field_descriptors s.descriptor) field)})
-  : Tot (s':array_struct u#a{s'.descriptor << s.descriptor})
-  =
-  let field_descriptors = Struct?.field_descriptors s.descriptor in
-  let Some sub_descriptor = field_descriptors field in
-  struct_field_type_unroll_lemma u#a s;
-  let sub_v = DepMap.sel u#a #_ #(struct_field_type field_descriptors) s.value field in
-  FStar.WellFounded.axiom1 field_descriptors field;
-  ArrayStruct sub_descriptor sub_v
-
-let rec composable_array_struct' (s0 s1: array_struct u#a) : Tot prop (decreases s0.descriptor) =
-  match s0.descriptor, s1.descriptor with
-  | Base a0 pcm0, Base a1 pcm1 ->
-    a0 == a1 /\ pcm0 == pcm1 /\
-    composable pcm0 s0.value s1.value
-  | Array descriptor0 len0, Array descriptor1 len1 ->
-    descriptor0 == descriptor1 /\ len0 == len1 /\
-    begin forall (i:nat{i < v_usize len0}).
-      {:pattern (array_cell_sub_array_struct s0 i) \/ (array_cell_sub_array_struct s1 i)}
-       composable_array_struct'
-         (array_cell_sub_array_struct s0 i)
-         (array_cell_sub_array_struct s1 i)
-    end
-  | Struct field_descriptors0, Struct field_descriptors1 ->
-    field_descriptors0 == field_descriptors1 /\
-    begin forall (field: field_id{Some? (field_descriptors0 field)}).
-      {:pattern (struct_field_sub_array_struct s0 field) \/ (struct_field_sub_array_struct s1 field)}
-      composable_array_struct'
-        (struct_field_sub_array_struct s0 field)
-        (struct_field_sub_array_struct s1 field)
-    end
-  | _ -> False
-
-
-let composable_array_struct_struct_case_intro
-  (s0: array_struct u#a{Struct? s0.descriptor})
-  (s1: array_struct u#a {Struct? s1.descriptor /\
-    Struct?.field_descriptors s0.descriptor == Struct?.field_descriptors s1.descriptor
-  })
-  (lemma: (field: field_id{Some? ((Struct?.field_descriptors s0.descriptor) field)}) -> Lemma (
-      composable_array_struct'
-        (struct_field_sub_array_struct s0 field)
-        (struct_field_sub_array_struct s1 field)
-  ))
-    : Lemma (composable_array_struct' s0 s1)
-  =
-  struct_field_type_unroll_lemma u#a s0;
-  struct_field_type_unroll_lemma u#a s1;
-  Classical.forall_intro lemma
-
-let composable_array_struct_struct_case_elim
-  (s0: array_struct{Struct? s0.descriptor})
-  (s1: array_struct{Struct? s1.descriptor /\ composable_array_struct' s0 s1})
-  (field: field_id{Some? ((Struct?.field_descriptors s0.descriptor) field)})
-    : Lemma (
-      Struct?.field_descriptors s0.descriptor == Struct?.field_descriptors s1.descriptor /\
-      composable_array_struct'
-        (struct_field_sub_array_struct s0 field)
-        (struct_field_sub_array_struct s1 field)
+let rec nested_pcm_to_pcm
+  (descriptor: array_struct_descriptor u#a)
+  (nested_pcm: array_struct_nested_pcm u#a{descriptor `nested_pcm_sync` nested_pcm})
+    : Tot (pcm (array_struct_type descriptor)) (decreases descriptor) =
+  match descriptor, nested_pcm with
+  | _, PBase _ pcm -> pcm
+  | DArray cell_descriptor _, PArray cell_type _ cell_nested_pcm array_pcm ->
+    array_pcm (nested_pcm_to_pcm cell_descriptor cell_nested_pcm)
+  | DStruct field_descriptors, PStruct field_types field_nested_pcms struct_pcm ->
+    assert(descriptor `nested_pcm_sync` nested_pcm);
+    assume(field_types == struct_field_type field_descriptors); // Why can't F* find this???
+    struct_field_type_unroll_lemma field_descriptors;
+    struct_pcm (fun field ->
+      FStar.WellFounded.axiom1 field_descriptors field;
+      nested_pcm_to_pcm (field_descriptors field) (field_nested_pcms field)
     )
-  =
-  ()
 
-let rec composable_symmetric (s0 s1: array_struct u#a)
-    : Lemma
-      (requires composable_array_struct' s0 s1)
-      (ensures composable_array_struct' s1 s0)
-      (decreases s0.descriptor)
-  =
-  match s0.descriptor, s1.descriptor with
-  | Base a0 pcm0, Base a1 pcm1 ->
-    ()
-  | Array descriptor0 len0, Array descriptor1 len1 ->
-    let aux (i:nat{i < v_usize len0}) : Lemma (
-       composable_array_struct'
-         (array_cell_sub_array_struct s1 i)
-         (array_cell_sub_array_struct s0 i)
-    ) =
-      composable_symmetric
-        (array_cell_sub_array_struct s0 i)
-        (array_cell_sub_array_struct s1 i)
-    in
-    Classical.forall_intro aux
-  | Struct field_descriptors0, Struct field_descriptors1 ->
-    let aux (field: field_id{Some? (field_descriptors0 field)}) : Lemma (
-       composable_array_struct'
-         (struct_field_sub_array_struct s1 field)
-         (struct_field_sub_array_struct s0 field)
-    ) =
-       composable_symmetric
-         (struct_field_sub_array_struct s0 field)
-         (struct_field_sub_array_struct s1 field)
-    in
-    Classical.forall_intro aux
-  | _ -> ()
+let composable_array_struct : symrel u#(a+1) (array_struct u#a) = fun (s0 s1: array_struct u#a) ->
+  s0.descriptor == s1.descriptor /\ s0.nested_pcm == s1.nested_pcm /\
+  composable (nested_pcm_to_pcm s0.descriptor s0.nested_pcm) s0.value s1.value
 
-
-unfold let composable_array_struct : symrel array_struct =
-  let aux (s0 s1: array_struct) : Lemma (
-    composable_array_struct' s0 s1 <==> composable_array_struct' s1 s0
-  ) =
-    let aux (_: squash (composable_array_struct' s0 s1)) : Lemma (composable_array_struct' s1 s0) =
-      composable_symmetric s0 s1
-    in
-    Classical.impl_intro aux;
-    let aux (_: squash (composable_array_struct' s1 s0)) : Lemma (composable_array_struct' s0 s1) =
-      composable_symmetric s1 s0
-    in
-    Classical.impl_intro aux
-  in
-  Classical.forall_intro_2 aux;
-  composable_array_struct'
-#set-options "--print_universes"
-
-let rec compose_array_struct
-  (s0 : array_struct u#a)
+let compose_array_struct
+  (s0: array_struct u#a)
   (s1: array_struct u#a{s0 `composable_array_struct` s1})
-    : Tot (s':array_struct u#a{s'.descriptor == s0.descriptor})
-      (decreases s0.descriptor)
+    : array_struct u#a
   =
-
-  match s0.descriptor, s1.descriptor with
-  | Base a0 pcm0, Base a1 pcm1 ->
-    ArrayStruct s0.descriptor (op pcm0 s0.value s1.value)
-  | Array descriptor0 len0, Array descriptor1 len1 ->
-    let new_val : Seq.lseq u#a (array_struct_type u#a descriptor0) (v_usize len0) =
-      Seq.init (v_usize len0) (fun i ->
-        let new_sub_array_struct : array_struct u#a =
-          compose_array_struct
-            (array_cell_sub_array_struct s0 i)
-            (array_cell_sub_array_struct s1 i)
-        in
-        let cell_val : array_struct_type u#a descriptor0 = new_sub_array_struct.value in
-        cell_val
-      )
-    in
-    ArrayStruct s0.descriptor new_val
-  | Struct field_descriptors0, Struct field_descriptors1 ->
-    let aux (field: field_id) : Tot (struct_field_type field_descriptors0 field) =
-      match field_descriptors0 field, field_descriptors1 field with
-      | None, None ->
-        // Here I chose the type to be False, but how to provide a value ?
-        Univ.raise_val u#0 u#a ()
-      | Some sub_descriptor0, Some sub_descriptor1 ->
-        let new_sub_array_struct : array_struct u#a =
-          compose_array_struct
-            (struct_field_sub_array_struct s0 field)
-            (struct_field_sub_array_struct s1 field)
-        in
-        let cell_val : struct_field_type u#a field_descriptors0 field =
-          new_sub_array_struct.value
-        in
-        cell_val
-    in
-    struct_field_type_unroll_lemma_aux u#a field_descriptors0;
-    let new_val : array_struct_type u#a s0.descriptor =
-      DepMap.create #_ #(struct_field_type field_descriptors0) aux
-    in
-    ArrayStruct s0.descriptor new_val
+  let new_val = op (nested_pcm_to_pcm s0.descriptor s0.nested_pcm) s0.value s1.value in
+  ArrayStruct s0.descriptor s0.nested_pcm new_val
 
 let unit_pcm' : pcm' u#a (Univ.raise_t u#0 u#a unit) = {
     composable = (fun _ _ -> True);
@@ -327,195 +188,24 @@ let unit_pcm : pcm u#a (Univ.raise_t u#0 u#a unit)  = {
   is_unit = (fun x -> higher_unit x)
 }
 
-let one_array_struct : array_struct u#a  =
-  ArrayStruct u#a (Base (Univ.raise_t unit) unit_pcm) (Univ.raise_val ())
+let array_struct_unit : array_struct u#a =
+  ArrayStruct
+    (DBase (Univ.raise_t u#0 u#a unit))
+    (PBase (Univ.raise_t u#0 u#a unit) unit_pcm)
+    (Univ.raise_val u#0 u#a ())
+
+#set-options "--print_universes --print_implicits"
 
 let array_struct_pcm' : pcm' u#(a+1) (array_struct u#a) = {
-  composable = composable_array_struct;
-  op = compose_array_struct;
-  one = one_array_struct
+  composable = composable_array_struct u#a;
+  op = compose_array_struct u#a;
+  one = array_struct_unit u#a;
 }
 
-open FStar.Tactics
-
-let compose_opaque (x: array_struct u#a) (y :array_struct u#a{x `composable_array_struct` y}) =
-  x `compose_array_struct` y
-
-let struct_field_sub_array_struct_opaque
-  (s: array_struct u#a{Struct? s.descriptor})
-  (field: field_id{Some? ((Struct?.field_descriptors s.descriptor) field)})
-  = struct_field_sub_array_struct s field
-
-
-let compose_struct_field_sub_array_struct_lemma (x y : array_struct u#a) (field: field_id)
-    : Lemma
-      (requires (
-        Struct? x.descriptor /\ x `composable_array_struct` y /\
-        Some? ((Struct?.field_descriptors x.descriptor) field)
-      ))
-      (ensures (
-         let xf = struct_field_sub_array_struct x field in
-         let yf = struct_field_sub_array_struct y field in
-         let xyf = struct_field_sub_array_struct (x `compose_array_struct` y) field in
-         xyf == xf `compose_array_struct` yf
-      ))
-  =
-  let xf = struct_field_sub_array_struct_opaque x field in
-  let yf = struct_field_sub_array_struct_opaque y field in
-  let xyf = struct_field_sub_array_struct (x `compose_array_struct` y) field in
-  match x.descriptor, y.descriptor, (x `compose_array_struct` y).descriptor with
-  | Struct fields, Struct fields', Struct fields'' ->
-    assert(fields == fields');
-    assert(fields == fields'');
-    assert(xf.descriptor == Some?.v (fields field));
-    assert(yf.descriptor == Some?.v (fields field));
-    assert(xyf.descriptor == Some?.v (fields field));
-    let xfyf = xf `compose_opaque` yf in
-    assert(xyf == xfyf) by begin
-      norm [delta_only ["Steel.PCM.ArrayStruct.Memory.compose_array_struct"]; zeta];
-      norm [nbe; simplify; weak; hnf];
-      // Here we just want the tactics engine to figure out that it can reduce the match...
-      tadmit ()
-    end;
-    admit()
-  | _ -> ()
-
-#push-options "--z3rlimit 20"
-let array_struct_assoc_l_helper
-  (x: array_struct u#a{Struct? x.descriptor})
-  (y: array_struct u#a)
-  (z: array_struct u#a{
-    y `composable_array_struct` z /\
-    x `composable_array_struct` (y `compose_array_struct` z)
-  })
-  (field: field_id{Some? (( Struct?.field_descriptors x.descriptor) field)})
-    : Lemma (requires (
-      let fields = Struct?.field_descriptors x.descriptor in
-      let xi = struct_field_sub_array_struct x field in
-      let yi = struct_field_sub_array_struct y field in
-      let zi = struct_field_sub_array_struct z field in
-      composable_array_struct yi zi /\ composable_array_struct xi (yi `compose_array_struct` zi)
-    ))
-    (ensures (
-      let fields = Struct?.field_descriptors x.descriptor in
-      struct_field_type_unroll_lemma_aux u#a fields;
-      let xi = struct_field_sub_array_struct x field in
-      let yi = struct_field_sub_array_struct y field in
-      let zi = struct_field_sub_array_struct z field in
-      (xi `compose_array_struct` (yi `compose_array_struct` zi)).value ==
-      FStar.DependentMap.sel
-        #field_id
-        #(struct_field_type (Struct?.field_descriptors x.descriptor))
-        (x `compose_array_struct` (y `compose_array_struct` z)).value field
-    ))
-  =
-  admit()
-
-
-#push-options "--z3rlimit 50 --warn_error -271"
-let rec arraystruct_assoc_l
-  (x:array_struct u#a)
-  (y:array_struct u#a)
-  (z:array_struct u#a)
-    : Lemma (requires (
-      composable_array_struct y z /\ composable_array_struct x (y `compose_array_struct` z)
-    )) (ensures (
-      composable_array_struct x y /\ composable_array_struct (x `compose_array_struct` y) z /\
-      x `compose_array_struct` (y `compose_array_struct` z) ==
-        (x `compose_array_struct` y) `compose_array_struct` z
-    )) (decreases x.descriptor)
-  =
-  match x.descriptor, y.descriptor, z.descriptor with
-  | Base _ pcm, Base _ _, Base _ _ ->
-    pcm.assoc x.value y.value z.value
-  | Array a len, Array _ _, Array _ _ ->
-    let aux (i:nat{i < v_usize len}) : Lemma (
-      let xi = array_cell_sub_array_struct x i in
-      let yi = array_cell_sub_array_struct y i in
-      let zi = array_cell_sub_array_struct z i in
-      composable_array_struct xi yi /\ composable_array_struct (xi `compose_array_struct` yi) zi /\
-      xi `compose_array_struct` (yi `compose_array_struct` zi) ==
-        (xi `compose_array_struct` yi) `compose_array_struct` zi
-    ) =
-      let xi = array_cell_sub_array_struct x i in
-      let yi = array_cell_sub_array_struct y i in
-      let zi = array_cell_sub_array_struct z i in
-      arraystruct_assoc_l xi yi zi
-    in
-    Classical.forall_intro aux;
-    let yz = y `compose_array_struct` z in
-    let xy = x `compose_array_struct` y in
-    assert(
-      (x `compose_array_struct` yz).value `Seq.equal #(array_struct_type a)`
-      (xy `compose_array_struct` z).value
-    )
-  | Struct fields, Struct _, Struct _ ->
-      let aux_helper (x y: array_struct u#a) (field: field_id)
-        : Lemma
-          (requires (
-            Struct? x.descriptor /\ x `composable_array_struct` y /\
-            Some? ((Struct?.field_descriptors x.descriptor) field)
-          ))
-          (ensures (
-             let xf = struct_field_sub_array_struct x field in
-             let yf = struct_field_sub_array_struct y field in
-             let xyf = struct_field_sub_array_struct (x `compose_array_struct` y) field in
-             xyf == xf `compose_array_struct` yf
-          )) [SMTPat ()]
-      =
-      compose_struct_field_sub_array_struct_lemma x y field
-    in
-    let aux1 (field: field_id{Some? (fields field)}) : Lemma (
-      let xi = struct_field_sub_array_struct x field in
-      let yi = struct_field_sub_array_struct y field in
-      let zi = struct_field_sub_array_struct z field in
-      composable_array_struct xi yi /\ composable_array_struct (xi `compose_array_struct` yi) zi /\
-      xi `compose_array_struct` (yi `compose_array_struct` zi) ==
-        (xi `compose_array_struct` yi) `compose_array_struct` zi
-    ) [SMTPat ()] =
-      let xi = struct_field_sub_array_struct x field in
-      let yi = struct_field_sub_array_struct y field in
-      let zi = struct_field_sub_array_struct z field in
-      let yzi = struct_field_sub_array_struct (y `compose_array_struct` z) field in
-      arraystruct_assoc_l xi yi zi
-    in
-    assert(composable_array_struct x y);
-    assert(composable_array_struct (x `compose_array_struct` y) z);
-    struct_field_type_unroll_lemma_aux u#a fields;
-    let aux2 (field: field_id) : Lemma (
-      FStar.DependentMap.sel #field_id #(struct_field_type fields)
-        (x `compose_array_struct` (y `compose_array_struct` z)).value field ==
-      FStar.DependentMap.sel #field_id #(struct_field_type fields)
-        ((x `compose_array_struct` y) `compose_array_struct` z).value field
-    ) =
-      let v1 =
-        FStar.DependentMap.sel #field_id #(struct_field_type fields)
-          (x `compose_array_struct` (y `compose_array_struct` z)).value field
-      in
-      let v2 =
-        FStar.DependentMap.sel #field_id #(struct_field_type fields)
-          ((x `compose_array_struct` y) `compose_array_struct` z).value field
-      in
-      match
-        fields field
-      with
-      | None ->
-        assert((struct_field_type fields) field == Univ.raise_t u#0 u#a unit);
-        higher_unit u#a v1; higher_unit u#a v2
-      | Some descr ->
-        assert((struct_field_type fields) field == array_struct_type descr);
-        aux1 field;
-        let xi = struct_field_sub_array_struct x field in
-        let yi = struct_field_sub_array_struct y field in
-        let zi = struct_field_sub_array_struct z field in
-        array_struct_assoc_l_helper x y z field;
-        // DM 04/21/2020: Why are these assumes still needed?
-        assume((xi `compose_array_struct` (yi `compose_array_struct` zi)).value == v1);
-        assume(((xi `compose_array_struct` yi) `compose_array_struct` zi).value == v2)
-    in
-    Classical.forall_intro aux2;
-    assert(
-      (x `compose_array_struct` (y `compose_array_struct` z)).value
-        `FStar.DependentMap.equal #field_id #(struct_field_type fields)`
-          ((x `compose_array_struct` y) `compose_array_struct` z).value
-    )
+let array_struct_pcm : pcm u#(a+1) (array_struct u#a) = {
+  p = array_struct_pcm' u#a;
+  comm = (fun _ _  -> admit());
+  assoc = (fun _ _ _ -> admit());
+  assoc_r = (fun _ _ _ -> admit());
+  is_unit = (fun x -> admit());
+}
